# 《一个组合恒等式的证明（补充）》`2024-10-05`

- 证明

$$
\sum_{m=0}^\infty\binom{m+k}{m}x^m=\frac{1}{(1-x)^{k+1}}
$$

- 我选择直接对右侧做泰勒展开

- 设

$$
f(x)=\frac{1}{(1-x)^{k+1}}
$$

- 我们需要计算 $f(x)$ 的在零处的各阶导数

$$
\begin{aligned}
f'(x)&=(k+1)\cdot \frac{1}{(1-x)^{k+2}}\\
f''(x)&=(k+1)(k+2)\cdot \frac{1}{(1-x)^{k+3}}\\
\cdots\\
f^{(t)}&=(k+1)(k+2)\cdots (k+t)\cdot \frac{1}{(1-x)^{k+t+1}}
\end{aligned}
$$

- 于是我们得到

$$
\begin{aligned}
f(x)&=\sum_{t=0}^{\infty}\frac{1}{t!}\cdot \frac{(k+t)!}{k!}\cdot x^t\\
&=\sum_{t=0}^\infty\binom{t+k}{t}x^t
\end{aligned}
$$

